\begin{align} 
\frac{\partial V}{\partial \phi_{d}} &= +\frac{1}{8} v_d \Big(4 g_{p}^{2} Q_{H_d} \Big(Q_{H_d} v_{d}^{2}  + Q_{H_u} v_{u}^{2}  + Q_s v_{S}^{2} \Big) + \Big(g_{1}^{2} + g_{2}^{2}\Big)\Big(- v_u  + v_d\Big)\Big(v_d + v_u\Big)\Big)\nonumber \\ 
 &+\frac{1}{2} \Big(- \sqrt{2} v_S v_u T_{\lambda}  + v_d \Big(2 m_{H_d}^2  + \Big(v_{S}^{2} + v_{u}^{2}\Big)\lambda^{2} \Big)\Big)\\ 
\frac{\partial V}{\partial \phi_{u}} &= +\frac{1}{8} v_u \Big(4 g_{p}^{2} Q_{H_u} \Big(Q_{H_d} v_{d}^{2}  + Q_{H_u} v_{u}^{2}  + Q_s v_{S}^{2} \Big) + \Big(g_{1}^{2} + g_{2}^{2}\Big)\Big(- v_{d}^{2}  + v_{u}^{2}\Big)\Big)\nonumber \\ 
 &+\frac{1}{2} \Big(- \sqrt{2} v_d v_S T_{\lambda}  + v_u \Big(2 m_{H_u}^2  + \Big(v_{d}^{2} + v_{S}^{2}\Big)\lambda^{2} \Big)\Big)\\ 
\frac{\partial V}{\partial \sigma_s} &= \frac{1}{2} g_{p}^{2} Q_s v_S \Big(Q_{H_d} v_{d}^{2}  + Q_{H_u} v_{u}^{2}  + Q_s v_{S}^{2} \Big) + \frac{1}{2} \Big(- \sqrt{2} v_d v_u T_{\lambda}  + v_S \Big(2 m^2_{s}  + \Big(v_{d}^{2} + v_{u}^{2}\Big)\lambda^{2} \Big)\Big)
\end{align} 
